Fix well_formed_preserved_by_deepcopy_replicaset

src/proof/apimodel.v
@@ -42,36 +42,52 @@ Context `{!auth_setG Σ KKey.t}.
 Definition mk_pod_key (namespace name: go_string) : KKey.t :=
   {| KKey.Kind' := "Pod"%go; KKey.Namespace' := namespace; KKey.Name' := name;|}.
 
+
 Definition extract_pod_key pod : KKey.t :=
   mk_pod_key pod.(v1.Pod.ObjectMeta').(v1.ObjectMeta.Namespace') pod.(v1.Pod.ObjectMeta').(v1.ObjectMeta.Name').
+
+
+Definition extract_kobject_metadata kobj : v1.ObjectMeta.t :=
+  match kobj with
+  | KObject.Pod p => p.(v1.Pod.ObjectMeta')
+  | KObject.ReplicaSet rs => rs.(v1.ReplicaSet.ObjectMeta')
+  end.
+
 
 Definition mk_replicaset_key (namespace name: go_string) : KKey.t :=
   {| KKey.Kind' := "ReplicaSet"%go; KKey.Namespace' := namespace; KKey.Name' := name;|}.
 
+Definition object_meta_well_formed (m: v1.ObjectMeta.t) : iProp Σ :=
+  ⌜ m.(v1.ObjectMeta.UID') ≠ "_ORPHAN_POD"%go ⌝.
 
 Definition pod_well_formed (pod: v1.Pod.t) : iProp Σ :=
-  True%I.
+  object_meta_well_formed pod.(v1.Pod.ObjectMeta').
 
 Definition pod_nn_well_formed (pod: v1.Pod.t) (namespace name: go_string) : iProp Σ :=
   ⌜ pod.(v1.Pod.ObjectMeta').(v1.ObjectMeta.Namespace') = namespace ⌝ ∗
   ⌜ pod.(v1.Pod.ObjectMeta').(v1.ObjectMeta.Name') = name ⌝ ∗
   pod_well_formed pod.
 
+Definition replicaset_well_formed (rs: v1.ReplicaSet.t) : iProp Σ :=
+  object_meta_well_formed rs.(v1.ReplicaSet.ObjectMeta') ∗
+  ∃ (v: w32), rs.(v1.ReplicaSet.Spec').(v1.ReplicaSetSpec.Replicas') ↦ v ∗ ⌜ 0 ≤ sint.Z v ⌝.
 
 Definition replicaset_nn_well_formed (rs: v1.ReplicaSet.t) (namespace name: go_string) : iProp Σ :=
- True%I.
+  ⌜ rs.(v1.ReplicaSet.ObjectMeta').(v1.ObjectMeta.Namespace') = namespace ⌝ ∗
+  ⌜ rs.(v1.ReplicaSet.ObjectMeta').(v1.ObjectMeta.Name') = name ⌝ ∗
+  replicaset_well_formed rs.
 
 Definition pod_rep k v1 v2 ptr pod : iProp Σ :=
   "%interface_is_pod_ptr" ∷ ⌜ v1 = interface.mk (ptrT.id v1.Pod.id) #ptr ⌝ ∗
   "pod_ptr" ∷ ptr ↦ pod ∗
   "%abs_v_is_pod" ∷ ⌜ v2 = KObject.Pod pod ⌝ ∗
-  "%pod_nn_well_formed" ∷ pod_nn_well_formed pod (KKey.Namespace' k) (KKey.Name' k).
+  "pod_nn_well_formed" ∷ pod_nn_well_formed pod (KKey.Namespace' k) (KKey.Name' k).
 
 Definition replicaset_rep k v1 v2 ptr rs : iProp Σ :=
   "%interface_is_rs_ptr" ∷ ⌜ v1 = interface.mk (ptrT.id v1.ReplicaSet.id) #ptr ⌝ ∗
   "rs_ptr" ∷ ptr ↦ rs ∗
   "%abs_v_is_rs" ∷ ⌜ v2 = KObject.ReplicaSet rs ⌝ ∗
-  "%replicaset_nn_well_formed" ∷ replicaset_nn_well_formed rs (KKey.Namespace' k) (KKey.Name' k).
+  "replicaset_nn_well_formed" ∷ replicaset_nn_well_formed rs (KKey.Namespace' k) (KKey.Name' k).
 
 Definition state_rep (phys_state: gmap KKey.t interface.t) (abs_state: gmap KKey.t KObject.t) : iProp Σ :=
   [∗ map] k ↦ v1; v2 ∈ phys_state; abs_state,
@@ -94,18 +110,60 @@ Definition is_kubernetes_state_inner γ_state γ_children γ_fresh_keys: iProp �
     "phys_abs_rep" ∷ state_rep phys_state abs_state ∗
     "own_children" ∷ map_ctx γ_children 1 children ∗
     "own_fresh_keys" ∷ auth_set_auth γ_fresh_keys fresh_keys ∗
-    "%consistent" ∷ ⌜ kubernetes_state_consistent abs_state children fresh_keys ⌝ .
+    "%consistent" ∷ ⌜ kubernetes_state_consistent abs_state children fresh_keys ⌝.
 
 
 Definition is_kubernetes_state γ_state γ_children γ_fresh_keys : iProp Σ :=
   is_Mutex (global_addr apimodel.stateMu) (is_kubernetes_state_inner γ_state γ_children γ_fresh_keys).
 
+Definition symmetric_iProp {A} (R : A → A → iProp Σ) :=
+  ∀ x y, R x y ⊣⊢ R y x.
+
 (* TODO: finish the deepcopy definition *)
-Definition is_deepcopy_pod (pod1 pod2: v1.Pod.t) : iProp Σ :=
+
+Definition deepcopy_of_w32_loc (src dst: loc) : iProp Σ :=
+  ⌜src = null ↔ dst = null⌝ ∧
+  ∀ (v1 v2: w32), src ↦ v1 -∗ dst ↦ v2 -∗ ⌜ v1 = v2 ⌝.
+
+Definition deepcopy_of_type_meta (src dst: v1.TypeMeta.t) : iProp Σ :=
+  ⌜ src = dst ⌝.
+
+Definition deepcopy_of_object_meta (src dst: v1.ObjectMeta.t) : iProp Σ :=
   True%I.
 
-Definition is_deepcopy_replicaset (rs1 rs2: v1.ReplicaSet.t) : iProp Σ :=
+Definition deepcopy_of_pod_spec (src dst: v1.PodSpec.t) : iProp Σ :=
   True%I.
+
+Definition deepcopy_of_pod_status (src dst: v1.PodStatus.t) : iProp Σ :=
+  True%I.
+
+Definition deepcopy_of_pod (src dst: v1.Pod.t) : iProp Σ :=
+  deepcopy_of_type_meta src.(v1.Pod.TypeMeta') dst.(v1.Pod.TypeMeta') ∗
+  deepcopy_of_object_meta src.(v1.Pod.ObjectMeta') dst.(v1.Pod.ObjectMeta') ∗
+  deepcopy_of_pod_spec src.(v1.Pod.Spec') dst.(v1.Pod.Spec') ∗
+  deepcopy_of_pod_status src.(v1.Pod.Status') dst.(v1.Pod.Status').
+
+Definition deepcopy_of_replicaset_spec (src dst: v1.ReplicaSetSpec.t) : iProp Σ :=
+  deepcopy_of_w32_loc src.(v1.ReplicaSetSpec.Replicas') dst.(v1.ReplicaSetSpec.Replicas').
+
+Definition deepcopy_of_replicaset_status (src dst: v1.ReplicaSetStatus.t) : iProp Σ :=
+  True%I.
+
+Definition deepcopy_of_replicaset (src dst: v1.ReplicaSet.t) : iProp Σ :=
+  deepcopy_of_type_meta src.(v1.ReplicaSet.TypeMeta') dst.(v1.ReplicaSet.TypeMeta') ∗
+  deepcopy_of_object_meta src.(v1.ReplicaSet.ObjectMeta') dst.(v1.ReplicaSet.ObjectMeta') ∗
+  deepcopy_of_replicaset_spec src.(v1.ReplicaSet.Spec') dst.(v1.ReplicaSet.Spec') ∗
+  deepcopy_of_replicaset_status src.(v1.ReplicaSet.Status') dst.(v1.ReplicaSet.Status').
+
+Lemma deepcopy_of_pod_symmetric:
+  symmetric_iProp deepcopy_of_pod.
+Proof.
+Admitted.
+
+Lemma deepcopy_of_replicaset_symmetric:
+  symmetric_iProp deepcopy_of_replicaset.
+Proof.
+Admitted.
 
 Definition pod_has_controller_parent_uid (pod: v1.Pod.t) (os: list v1.OwnerReference.t) (o: v1.OwnerReference.t) (c: bool) : iProp Σ :=
   pod.(v1.Pod.ObjectMeta').(v1.ObjectMeta.OwnerReferences') ↦* os ∗
@@ -113,13 +171,15 @@ Definition pod_has_controller_parent_uid (pod: v1.Pod.t) (os: list v1.OwnerRefer
   o.(v1.OwnerReference.Controller') ↦ c ∗
   ⌜ c = true ⌝.
 
-Definition index_is_pod_controller_uid_index (pod: v1.Pod.t) (index: go_string): iProp Σ :=
-  (∃ os o c, pod_has_controller_parent_uid pod os o c ∗ ⌜ o.(v1.OwnerReference.UID') = index ⌝) ∨
-  (¬(∃ os o c, pod_has_controller_parent_uid pod os o c) ∗ ⌜ index = "_ORPHAN_POD"%go ⌝).
+Definition is_pod_controller_uid_index (pod: v1.Pod.t) (indexed_value: go_string): iProp Σ :=
+  (∃ os o c, pod_has_controller_parent_uid pod os o c ∗ ⌜ o.(v1.OwnerReference.UID') = indexed_value ⌝) ∨
+  (¬(∃ os o c, pod_has_controller_parent_uid pod os o c) ∗ ⌜ indexed_value = "_ORPHAN_POD"%go ⌝).
 
 Lemma well_formed_preserved_by_deepcopy_replicaset rs1 rs2 namespace name:
-  is_deepcopy_replicaset rs1 rs2 -∗
+  deepcopy_of_replicaset rs1 rs2 -∗
     replicaset_nn_well_formed rs1 namespace name -∗
+      deepcopy_of_replicaset rs1 rs2 ∗
+      replicaset_nn_well_formed rs1 namespace name ∗
       replicaset_nn_well_formed rs2 namespace name.
 Proof.
 Admitted.
@@ -143,10 +203,10 @@ Lemma wp_deepCopy_replicaset (obj: interface.t) (ptr: loc) (rs: v1.ReplicaSet.t)
   }}}
     @! apimodel.deepCopy #obj
   {{{ (obj': interface.t) (ptr': loc) (rs': v1.ReplicaSet.t), RET #obj';
-    ⌜ obj' = interface.mk (ptrT.id v1.ReplicaSet.id) #ptr' ⌝ ∗
-    ptr' ↦ rs' ∗
-    is_deepcopy_replicaset rs rs' ∗
-    ptr ↦ rs
+      ⌜ obj' = interface.mk (ptrT.id v1.ReplicaSet.id) #ptr' ⌝ ∗
+      ptr' ↦ rs' ∗
+      deepcopy_of_replicaset rs rs' ∗
+      ptr ↦ rs
   }}}.
 Proof.
 Admitted.
@@ -157,7 +217,7 @@ Lemma wp_objGet (key: KKey.t) γ_state γ_children γ_fresh_keys:
   }}}
     @! apimodel.objGet #key
   {{{ (obj: interface.t) (exists': bool), RET (#obj, #exists');
-    True
+      True
   }}}.
 Proof.
   wp_start as "H". iNamed "H".
@@ -185,10 +245,10 @@ Lemma wp_PodGet (namespace name: go_string) γ_state γ_children γ_fresh_keys:
   }}}
     @! apimodel.PodGet #namespace #name
   {{{ (l: loc) (err: error.t) dq2 (pod: v1.Pod.t), RET (#l, #err);
-    if decide (err = interface.nil) then
-      l ↦{dq2} pod
-    else
-      True
+      if decide (err = interface.nil) then
+        l ↦{dq2} pod
+      else
+        True
   }}}.
 Proof.
 Admitted.
@@ -200,11 +260,11 @@ Lemma wp_podControllerUIDIndex_with_controller_parent obj ptr pod:
       "ptr" ∷ ptr ↦ pod
   }}}
     @! apimodel.podControllerUIDIndex #obj
-  {{{ indexes (err: error.t) vs index, RET (#indexes, #err);
-    ⌜ err = interface.nil ⌝ ∗
-    indexes ↦* vs ∗
-    ⌜ vs = [index] ⌝ ∗
-    index_is_pod_controller_uid_index pod index
+  {{{ indexed_values (err: error.t) indexed_value_list indexed_value, RET (#indexed_values, #err);
+      ⌜ err = interface.nil ⌝ ∗
+      indexed_values ↦* indexed_value_list ∗
+      ⌜ indexed_value_list = [indexed_value] ⌝ ∗
+      is_pod_controller_uid_index pod indexed_value
   }}}.
 Proof.
 Admitted.
@@ -215,22 +275,53 @@ Lemma wp_objList_pod_ptsto_mut kind namespace γ_state γ_children γ_fresh_keys
       "own_pods" ∷ ([∗ map] key ↦ pod ∈ owned_pod_map, key [[ γ_state ]]↦ KObject.Pod pod) ∗
       "%kind" ∷ ⌜ kind = "Pod"%go ⌝
   }}}
-  @! apimodel.objList #kind #namespace
+    @! apimodel.objList #kind #namespace
   {{{ (l: slice.t) (objs: list interface.t) (pods: list v1.Pod.t), RET #l;
-    l ↦* objs ∗
-    ⌜ NoDup (map extract_pod_key pods) ⌝ ∗
-    ([∗ list] obj ; pod ∈ objs ; pods, ∃ (ptr : loc),
-      ⌜ obj = interface.mk (ptrT.id v1.ReplicaSet.id) #ptr ⌝ ∗
-      ptr ↦ pod ∗
-      pod_well_formed pod ∗
-      ⌜ namespace = ""%go ∨ pod.(v1.Pod.ObjectMeta').(v1.ObjectMeta.Namespace') = namespace ⌝
-    ) ∗
-    ([∗ map] key ↦ owned_pod ∈ owned_pod_map,
-      if bool_decide (namespace = ""%go ∨ key.(KKey.Namespace') = namespace)
-      then ∃ pod, ⌜ pod ∈ pods ⌝ ∗ is_deepcopy_pod owned_pod pod
-      else ∀ pod, ⌜ pod ∈ pods → key ≠ extract_pod_key pod ⌝
-    ) ∗
-    ([∗ map] key ↦ pod ∈ owned_pod_map, key [[ γ_state ]]↦ KObject.Pod pod)
+      l ↦* objs ∗
+      ⌜ NoDup (map extract_pod_key pods) ⌝ ∗
+      ([∗ list] obj ; pod ∈ objs ; pods, ∃ (ptr : loc),
+        ⌜ obj = interface.mk (ptrT.id v1.ReplicaSet.id) #ptr ⌝ ∗
+        ptr ↦ pod ∗
+        pod_well_formed pod ∗
+        ⌜ namespace = ""%go ∨ pod.(v1.Pod.ObjectMeta').(v1.ObjectMeta.Namespace') = namespace ⌝
+      ) ∗
+      ([∗ map] key ↦ owned_pod ∈ owned_pod_map,
+        if bool_decide (namespace = ""%go ∨ key.(KKey.Namespace') = namespace)
+        then ∃ pod, ⌜ pod ∈ pods ⌝ ∗ deepcopy_of_pod owned_pod pod
+        else ∀ pod, ⌜ pod ∈ pods → key ≠ extract_pod_key pod ⌝
+      ) ∗
+      ([∗ map] key ↦ pod ∈ owned_pod_map, key [[ γ_state ]]↦ KObject.Pod pod)
+  }}}.
+Proof.
+Admitted.
+
+
+Lemma wp_ByIndex_pod_ptsto_mut kind index_name indexed_value γ_state γ_children γ_fresh_keys parent_key owned_parent owned_pod_map owned_child_keys:
+  {{{ is_pkg_init apimodel ∗
+      "#inv" ∷ is_kubernetes_state γ_state γ_children γ_fresh_keys ∗
+      "own_parent" ∷ parent_key [[ γ_state ]]↦ owned_parent ∗
+      "own_pods" ∷ ([∗ map] key ↦ pod ∈ owned_pod_map, key [[ γ_state ]]↦ KObject.Pod pod) ∗
+      "own_child_keys" ∷ parent_key [[ γ_children ]]↦ owned_child_keys ∗
+      "%owned_child_keys_equal_dom_owned_pods" ∷ ⌜ owned_child_keys = dom owned_pod_map ⌝ ∗
+      "%indexed_value" ∷ ⌜ indexed_value = (extract_kobject_metadata owned_parent).(v1.ObjectMeta.UID') ⌝ ∗
+      "%kind" ∷ ⌜ kind = "Pod"%go ⌝ ∗
+      "%index_name" ∷ ⌜ index_name = "podControllerUID"%go ⌝
+  }}}
+    @! apimodel.ByIndex #kind #index_name #indexed_value
+  {{{ (l: slice.t) (err: error.t) (objs: list interface.t) (pods: list v1.Pod.t), RET #l;
+      l ↦* objs ∗
+      ⌜ NoDup (map extract_pod_key pods) ⌝ ∗
+      ([∗ list] obj ; pod ∈ objs ; pods, ∃ (ptr : loc),
+        ⌜ obj = interface.mk (ptrT.id v1.ReplicaSet.id) #ptr ⌝ ∗
+        ptr ↦ pod ∗
+        pod_well_formed pod ∗
+        is_pod_controller_uid_index pod indexed_value
+      ) ∗
+      ⌜ Forall (λ pod, owned_pod_map !! extract_pod_key pod = Some pod) pods ⌝ ∗
+      ⌜ dom owned_pod_map = list_to_set (extract_pod_key <$> pods) ⌝ ∗
+      parent_key [[ γ_state ]]↦ owned_parent ∗
+      ([∗ map] key ↦ pod ∈ owned_pod_map, key [[ γ_state ]]↦ KObject.Pod pod) ∗
+      parent_key [[ γ_children ]]↦ owned_child_keys
   }}}.
 Proof.
 Admitted.
@@ -244,14 +335,14 @@ Lemma wp_objGet_replicaset_ptsto_mut key γ_state γ_children γ_fresh_keys owne
   }}}
     @! apimodel.objGet #key
   {{{ obj exists' rs, RET (#obj, #exists');
-    ⌜ exists' = true ⌝ ∗
-    (∃ (ptr : loc),
-        ⌜ obj = interface.mk (ptrT.id v1.ReplicaSet.id) #ptr ⌝ ∗
-        ptr ↦ rs
-    ) ∗
-    is_deepcopy_replicaset owned_rs rs ∗
-    replicaset_nn_well_formed rs (KKey.Namespace' key) (KKey.Name' key) ∗
-    key [[ γ_state ]]↦ (KObject.ReplicaSet owned_rs)
+      ⌜ exists' = true ⌝ ∗
+      (∃ (ptr : loc),
+          ⌜ obj = interface.mk (ptrT.id v1.ReplicaSet.id) #ptr ⌝ ∗
+          ptr ↦ rs
+      ) ∗
+      deepcopy_of_replicaset owned_rs rs ∗
+      replicaset_nn_well_formed rs (KKey.Namespace' key) (KKey.Name' key) ∗
+      key [[ γ_state ]]↦ (KObject.ReplicaSet owned_rs)
   }}}.
 Proof.
   wp_start as "H". iNamed "H".
@@ -285,13 +376,10 @@ Proof.
   wp_apply (wp_deepCopy_replicaset with "[$rs_ptr]").
   { iPureIntro. reflexivity. }
   iIntros (obj' ptr' rs') "(%obj'_is_ptr & ptr' & rs'_is_deepcopy_of_rs & rs_ptr)".
-  iAssert (replicaset_nn_well_formed rs' (KKey.Namespace' key) (KKey.Name' key)%I) with "[rs'_is_deepcopy_of_rs]" as "%rs'_well_formed".
-  {
-    iApply (well_formed_preserved_by_deepcopy_replicaset with "[$rs'_is_deepcopy_of_rs]").
-    iPureIntro. done.
-  }
+  iPoseProof (well_formed_preserved_by_deepcopy_replicaset owned_rs rs' (KKey.Namespace' key) (KKey.Name' key)
+  with "[$rs'_is_deepcopy_of_rs] [$replicaset_nn_well_formed]") as "(rs'_is_deepcopy_of_rs & replicaset_nn_well_formed & rs'_nn_well_formed)".
   wp_auto.
-  iAssert (state_rep phys_state abs_state %I) with "[rs_ptr other_rep]" as "phys_abs_rep".
+  iAssert (state_rep phys_state abs_state %I) with "[rs_ptr other_rep replicaset_nn_well_formed]" as "phys_abs_rep".
   { iApply "other_rep". iExists ptr, owned_rs. iFrame. done. }
   wp_apply (wp_Mutex__Unlock _ (is_kubernetes_state_inner γ_state γ_children γ_fresh_keys)
   with "[$own_Mutex state_m_addr own_phys own_abs phys_abs_rep own_children own_fresh_keys]").
@@ -310,17 +398,17 @@ Lemma wp_ReplicaSetMutGet_ptsto_mut namespace name γ_state γ_children γ_fresh
   }}}
     @! apimodel.ReplicaSetMutGet #namespace #name
   {{{ l (err: error.t) rs, RET (#l, #err);
-    ⌜ err = interface.nil ⌝ ∗
-    (mk_replicaset_key namespace name) [[ γ_state ]]↦ (KObject.ReplicaSet owned_rs) ∗
-    l ↦ rs ∗
-    is_deepcopy_replicaset owned_rs rs ∗
-    replicaset_nn_well_formed rs namespace name
+      ⌜ err = interface.nil ⌝ ∗
+      (mk_replicaset_key namespace name) [[ γ_state ]]↦ (KObject.ReplicaSet owned_rs) ∗
+      l ↦ rs ∗
+      deepcopy_of_replicaset owned_rs rs ∗
+      replicaset_nn_well_formed rs namespace name
   }}}.
 Proof.
   wp_start as "H". iNamed "H". wp_auto.
   wp_apply (wp_objGet_replicaset_ptsto_mut with "[$own_rs]").
   { iFrame "#". done. }
-  iIntros (obj exists' rs') "(%exists'_is_true & (%ptr & %obj_is_ptr & ptr) & deepcopy & %well_formed & own_rs)".
+  iIntros (obj exists' rs') "(%exists'_is_true & (%ptr & %obj_is_ptr & ptr) & deepcopy & well_formed & own_rs)".
   subst exists' obj.
   wp_auto.
   unshelve wp_apply wp_interface_checked_type_assert; try tc_solve.
@@ -345,17 +433,17 @@ Lemma wp_ReplicaSetGet_ptsto_mut namespace name γ_state γ_children γ_fresh_ke
   }}}
     @! apimodel.ReplicaSetGet #namespace #name
   {{{ l (err: error.t) rs dq, RET (#l, #err);
-    ⌜ err = interface.nil ⌝ ∗
-    (mk_replicaset_key namespace name) [[ γ_state ]]↦ (KObject.ReplicaSet owned_rs) ∗
-    l ↦{dq} rs ∗
-    is_deepcopy_replicaset owned_rs rs ∗
-    replicaset_nn_well_formed owned_rs namespace name
+      ⌜ err = interface.nil ⌝ ∗
+      (mk_replicaset_key namespace name) [[ γ_state ]]↦ (KObject.ReplicaSet owned_rs) ∗
+      l ↦{dq} rs ∗
+      deepcopy_of_replicaset owned_rs rs ∗
+      replicaset_nn_well_formed rs namespace name
   }}}.
 Proof.
   wp_start as "H". iNamed "H". wp_auto.
   wp_apply (wp_ReplicaSetMutGet_ptsto_mut with "[$own_rs]").
   { done. }
-  iIntros (l err rs') "(%err_is_nil & own_rs & l & deepcopy & %well_formed)".
+  iIntros (l err rs') "(%err_is_nil & own_rs & l & deepcopy & well_formed)".
   wp_auto.
   iApply "HΦ". iFrame. done.
 Qed.
